Define applyWithdrawals

EvmYul/State/Withdrawal.lean
@@ -2,38 +2,48 @@
 
 import EvmYul.Wheels
 import EvmYul.PerformIO
+import EvmYul.Maps.YPState
 import Conform.Wheels
+import EvmYul.EVM.Exception
 
 open EvmYul ByteArray
 
+/--
+EIP-4895: Beacon chain push withdrawals as operations.
+- `index` - starting from `0`
+- `validator_index`
+- `address` - a recipient for the withdrawn ether
+- `amount` - a nonzero amount of ether given in Gwei
+-/
 structure Withdrawal where
   index : UInt64
   validatorIndex : UInt64
-  recipient : Address
+  address : Address
   amount : UInt64
+deriving Repr
 
 namespace Withdrawal
 
 def to𝕋 : Withdrawal → 𝕋
-  | {index, validatorIndex, recipient, amount} =>
+  | {index, validatorIndex, address, amount} =>
     .𝕃
       [ .𝔹 (BE index.val.val)
       , .𝔹 (BE validatorIndex.val.val)
-      , .𝔹 (recipient.toByteArray)
+      , .𝔹 (address.toByteArray)
       , .𝔹 (BE amount.val.val)
       ]
 
 end Withdrawal
 
-def blobComputeTrieRoot (ws : List (String × String)) : String :=
+def blobComputeTrieRoot (ws : Array (String × String)) : String :=
   totallySafePerformIO ∘ IO.Process.run <|
     pythonCommandOfInput ws
-  where pythonCommandOfInput (ws : List (String × String)) : IO.Process.SpawnArgs := {
+  where pythonCommandOfInput (ws : Array (String × String)) : IO.Process.SpawnArgs := {
     cmd := "python3",
     args :=
       #["EvmYul/EllipticCurvesPy/withdrawal.py"]
-        ++ #[ws.length.repr]
-        ++ .mk (List.join ∘ List.map (λ (i, w) ↦ [i, w]) <| ws)
+        ++ #[ws.size.repr]
+        ++ (ws.map (λ (i, w) ↦ #[i, w])).join
   }
 
 def toBlobs (w : Withdrawal) : Option (String × String) := do
@@ -42,43 +52,65 @@ def toBlobs (w : Withdrawal) : Option (String × String) := do
   pure (EvmYul.toHex rlpᵢ, EvmYul.toHex rlp)
 
 -- EIP-4895
-def computeTrieRoot (ws : List Withdrawal) : Except String ByteArray := do
-  match List.traverse toBlobs ws with
+def computeTrieRoot (ws : Array Withdrawal) : Except String ByteArray := do
+  match Array.mapM toBlobs ws with
     | none => .error "Could not encode withdrawal."
     | some ws => ByteArray.ofBlob (blobComputeTrieRoot ws)
+
+def applyWithdrawals
+  (σ : YPState)
+  (withdrawalsRoot : ByteArray)
+  (ws : Array Withdrawal)
+    :
+  Except EVM.Exception YPState
+:=
+  match computeTrieRoot ws with
+    | .error e => .error (.InvalidWithdrawal e)
+    | .ok root => do
+      if root != withdrawalsRoot
+        then .error (.InvalidWithdrawal "Invalid withdrawals root.")
+      .ok <| ws.foldl applyWithdrawal σ
+ where
+  applyWithdrawal (σ : YPState) (w : Withdrawal) : YPState :=
+    if w.amount <= 0 then σ else
+      match σ.find? w.address with
+        | none =>
+          σ.insert w.address {(default : Account) with balance := w.amount.val.val * 10^9}
+        | some ac =>
+          σ.insert w.address {ac with balance := ac.balance + w.amount.val.val * 10^9}
 
 -- Tests
 
 private def withdrawal₁ : Withdrawal :=
   { index := 0x00
   , validatorIndex := 0x00
-  , recipient := 0x6295ee1b4f6dd65047762f924ecd367c17eabf8f
+  , address := 0x6295ee1b4f6dd65047762f924ecd367c17eabf8f
   , amount := 0x01
   }
 
 private def withdrawal₂ : Withdrawal :=
   { index := 0x00
   , validatorIndex := 0x00
-  , recipient := 0x000f3df6d732807ef1319fb7b8bb8522d0beac02
+  , address := 0x000f3df6d732807ef1319fb7b8bb8522d0beac02
   , amount := 0x01
   }
 
 private def withdrawal₃ : Withdrawal :=
   { index := 0x01
   , validatorIndex := 0x01
-  , recipient := 0xfffffffffffffffffffffffffffffffffffffffe
+  , address := 0xfffffffffffffffffffffffffffffffffffffffe
   , amount := 0x01
   }
 
 private def withdrawalZeroTrailingRoot : Withdrawal :=
   { index := 0x00
   , validatorIndex := 0x00
-  , recipient := 0x0000000000000000000000000000000000000001
+  , address := 0x0000000000000000000000000000000000000001
   , amount := 0x00
   }
 
 private example :
-  (computeTrieRoot []).toOption
+  (computeTrieRoot #[]).toOption
     ==
   (ByteArray.ofBlob
     "56e81f171bcc55a6ff8345e692c0f86e5b48e01b996cadc001622fb5e363b421"
@@ -87,7 +119,7 @@ private example :
 
 /- From newly_created_contract.json -/
 private example :
-  (computeTrieRoot [withdrawal₁]).toOption
+  (computeTrieRoot #[withdrawal₁]).toOption
     =
   (ByteArray.ofBlob
     "82cc6fbe74c41496b382fcdf25216c5af7bdbb5a3929e8f2e61bd6445ab66436"
@@ -96,7 +128,7 @@ private example :
 
 /- From beacon_root_contract_deploy.json -/
 private example :
-  (computeTrieRoot [withdrawal₂, withdrawal₃]).toOption
+  (computeTrieRoot #[withdrawal₂, withdrawal₃]).toOption
     =
   (ByteArray.ofBlob
     "2aef4d3e6939af0b4bf4c0e7572a214eb7db9ba52937e1e82ad6c64b52d2e8bb"
@@ -105,7 +137,7 @@ private example :
 
 /- From withdrawing_to_precompiles.json -/
 private example :
-  (computeTrieRoot [withdrawalZeroTrailingRoot]).toOption
+  (computeTrieRoot #[withdrawalZeroTrailingRoot]).toOption
     =
   (ByteArray.ofBlob
     "04cc2e3f94b587ff46b5f4c0787c589db306b7209f7f212f47022a12bc3e6e16"
