EvmYul/State/AccountOps.lean
@@ -82,7 +82,7 @@ section RemoveLater
 --   s!"ACCOUNT: [nonce: {acc.nonce}; balance: {acc.balance}; code: {acc.code.toList.take 5}...; codehash: {acc.codeHash}; storage: {stringOfStorage acc.storage}]; tstorage: {stringOfStorage acc.tstorage}"⟩
 
 instance : ToString Account := ⟨λ acc ↦
-  s!"ACCOUNT: storage: {repr acc.storage}]"⟩
+  s!"ACCOUNT: storage: {repr acc.storage}"⟩
 
 instance : Repr Account := ⟨λ acc _ ↦ ToString.toString acc⟩
 
